move to Power.dfy

montgomery.dfy
@@ -1,4 +1,8 @@
+include "Powers.dfy"
+
 module MONTGOMERY {
+    import opened Powers
+
     predicate congruent_def(a: int, b: int, n: int)
     {
         exists k : int :: a - b == n * k
@@ -820,31 +824,6 @@ module MONTGOMERY {
         ensures ((a % n) * b) % n == (a * b) % n;
     {
         not_so_interesting_lemma(a % n, a, b, n);
-    }
-
-    function method {:opaque} power(b:int, e:nat) : int
-        decreases e;
-    {
-        if (e == 0) then 1
-        else b * power(b, e - 1)
-    }
-
-    lemma {:induction e} power_base_one_lema(e: nat) 
-        ensures power(1, e) == 1;
-    {
-        reveal power();
-    }
-
-    lemma {:induction e} power_add_one_lema(b:int, e:nat)
-        ensures power(b, e) * b == power(b, e + 1);
-    {
-        reveal power();
-    }
-
-    lemma power_same_exp_lema(a: int, b: int, e: nat)
-        ensures power(a, e) * power(b, e) == power(a * b, e);
-    {
-        assume false;
     }
 
     lemma power_exp_lemma(a: nat, b: nat, n: nat)
