Powers.dfy
@@ -1,0 +1,27 @@
+module Powers
+{
+    function method {:opaque} power(b:int, e:nat) : int
+        decreases e;
+    {
+        if (e == 0) then 1
+        else b * power(b, e - 1)
+    }
+
+    lemma {:induction e} power_base_one_lema(e: nat) 
+        ensures power(1, e) == 1;
+    {
+        reveal power();
+    }
+
+    lemma {:induction e} power_add_one_lema(b:int, e:nat)
+        ensures power(b, e) * b == power(b, e + 1);
+    {
+        reveal power();
+    }
+
+    lemma power_same_exp_lema(a: int, b: int, e: nat)
+        ensures power(a, e) * power(b, e) == power(a * b, e);
+    {
+        assume false;
+    }
+}
